move the prog_environ definitions to separate files
this allows importing them without importing the language weakestpre

theories/language/weakestpre.v
@@ -1,6 +1,6 @@
 From iris.proofmode Require Import base proofmode classes.
 From iris.base_logic.lib Require Export fancy_updates.
-From melocoton.language Require Export language.
+From melocoton.language Require Export language progenv.
 (* FIXME: If we import iris.bi.weakestpre earlier texan triples do not
    get pretty-printed correctly. *)
 From iris.bi Require Export weakestpre.
@@ -47,19 +47,6 @@ Proof.
   rewrite /wp_pre /= => n wp wp' Hwp E e1 Φ. cbn in Hwp.
   repeat (f_contractive || f_equiv || apply Hwp || intros ?).
 Qed.
-
-Definition program_specification `{!langGS val Λ Σ, !invGS_gen hlc Σ} :=
-  string -d> list val -d> (val -d> iPropO Σ) -d> iPropO Σ.
-
-Record prog_environ {val} (Λ : language val) Σ := Penv {
-  penv_prog : gmap string Λ.(func);
-  penv_proto : string -d> list val -d> (val -d> iPropO Σ) -d> iPropO Σ;
-}.
-Global Arguments Penv {_ _ _} _ _.
-Global Arguments penv_prog {_ _ _} _.
-Global Arguments penv_proto {_ _ _} _.
-
-Notation "⟨ p , T ⟩" := (Penv p T : prog_environ _ _).
 
 Local Definition wp_def `{!langGS val Λ Σ, !invGS_gen hlc Σ} : Wp (iProp Σ) (expr Λ) val (prog_environ Λ Σ) :=
   λ p : (prog_environ Λ Σ), fixpoint (wp_pre p.(penv_prog) p.(penv_proto)).
