theories/language/progenv.v
@@ -1,0 +1,14 @@
+From iris.proofmode Require Import base.
+From iris.base_logic.lib Require Import fancy_updates.
+From melocoton.language Require Export language.
+From iris.prelude Require Import options.
+
+Record prog_environ {val} (Λ : language val) Σ := Penv {
+  penv_prog : gmap string Λ.(func);
+  penv_proto : string -d> list val -d> (val -d> iPropO Σ) -d> iPropO Σ;
+}.
+Global Arguments Penv {_ _ _} _ _.
+Global Arguments penv_prog {_ _ _} _.
+Global Arguments penv_proto {_ _ _} _.
+
+Notation "⟨ p , T ⟩" := (Penv p T : prog_environ _ _).
